:wrench: add part 2

part2.dfy
@@ -1,22 +1,126 @@
 /*
-  Part 2: Formally verified implementations
+  Part 2: Design by Contract
 
   In this part, we will give you the pre/postconditions
-  for several functions. Your job is to implement the
+  for several methods. Your job is to implement the
   function so that the verification passes.
 
-  ===== Grading requirements =====
+  Requirements:
+  - Since the specs are already written, the only requirement
+    is that you implement the methods so that the specs pass.
 
-  Your code should pass the Dafny verifier:
-    dafny part2.dfy
-  should pass with every function verified, no errors.
-  You can also simply check that the green bar shows up next
-  to every function in VSCode, throughout the whole file,
-  with no errors (shown in red).
+  - Don't change the function signatures or pre/postconditions
+    for any of the methods. You can add helper functions if needed.
+
+  - You will need to use loop invariants for 1 and 2.
+
+  - Your code should pass the Dafny verifier:
+      dafny verify part2.dfy
+    should pass with no errors or warnings.
+
+    You can also simply check that the green bar shows up next
+    to every function in VSCode, throughout the whole file,
+    with no errors (shown in red).
 */
 
-method TodoPlaceholder(a: int, b: int) returns (c: int)
+/*
+  1. Integer square root
+
+  This function should find the integer square root of a number:
+  the largest integer whose square is less than or equal to n.
+  For example, IntSqrt(3) == 1, IntSqrt(4) == 2, IntSqrt(5) == 2.
+*/
+
+method IntSqrt(n: int) returns (root: int)
+  requires n >= 0
+  ensures root * root <= n < (root + 1) * (root + 1)
+  // TODO: delete the following line and implement the function
   requires false
 {
   // TODO
+}
+
+/*
+  2. Number of digits function
+
+  Calculates the number of digits of a number (in base 10).
+
+  For example, NumDigits(123) == 3, NumDigits(1) == 1.
+*/
+
+// This function is used in the postcondition
+function pow(base: int, exponent: nat): int
+{
+  if exponent == 0 then 1 else base * pow(base, exponent - 1)
+}
+
+method NumDigits(n: int) returns (digits: int)
+  requires n >= 1
+  ensures digits >= 1
+  ensures pow(10, digits - 1) <= n < pow(10, digits)
+  // TODO: delete the following line and implement the function
+  requires false
+{
+  // TODO
+}
+
+/*
+  3. Function to increment a stopwatch
+
+  The last function assumes that we have a stopwatch that
+  stores the time as a number of seconds, minutes, hours, and days.
+
+  The function AdvanceStopwatch increments the stopwatch by a given
+  number of seconds, and returns the new values.
+*/
+
+function calc_seconds(
+  seconds: int, minutes: int, hours: int, days: int
+): int
+{
+  86400 * days + 3600 * hours + 60 * minutes + seconds
+}
+
+function stopwatch_invariant(
+  seconds: int, minutes: int, hours: int, days: int
+): bool
+{
+  0 <= seconds < 60 && 0 <= minutes < 60 && 0 <= hours < 24 && days >= 0
+}
+
+method AdvanceStopwatch(
+  seconds: int, minutes: int, hours: int, days: int,
+  advance_by: int
+) returns (new_seconds: int, new_minutes: int, new_hours: int, new_days: int)
+  requires stopwatch_invariant(seconds, minutes, hours, days)
+  ensures stopwatch_invariant(new_seconds, new_minutes, new_hours, new_days)
+  ensures calc_seconds(new_seconds, new_minutes, new_hours, new_days)
+       == calc_seconds(seconds, minutes, hours, days) + advance_by
+  // TODO: delete the following line and implement the function
+  requires false
+{
+  // TODO
+}
+
+/*
+  4. Uncomment the following tests to make sure that
+  your implementations are working.
+*/
+
+method Tests()
+{
+  // var x1 := IntSqrt(3);
+  // var x2 := IntSqrt(4);
+  // var x3 := IntSqrt(5);
+  // assert x1 == 1;
+  // assert x2 == 2;
+  // assert x3 == 2;
+
+  // var y1 := NumDigits(123);
+  // var y2 := NumDigits(1);
+  // assert y1 == 3;
+  // assert y2 == 1;
+
+  // var s, m, h, d := AdvanceStopwatch(0, 0, 0, 0, 65);
+  // assert s == 5 && m == 1 && h == 0 && d == 0;
 }
